

# Mathematical Modelling of a Rotary Inverted Pendulum (Furuta)

January 21, 2026

## 1. Definition

Generalized coordinates:

$\theta(t)$ : arm yaw angle.

$\alpha(t)$ : pendulum angle, with  $\alpha = 0$  upright.

Constants:

$L_r$ : arm length.

$m_p$ : swinging mass.

$l_p$ : distance from hinge to pendulum COM.

$g$ : gravity.

$\tau$ : actuation torque about  $\theta$ .

Define

$$K \equiv m_p L_r l_p, \quad G \equiv m_p g l_p$$

Let

$\hat{J}_1$ : yaw inertia about motor axis (arm-side).

$\hat{J}_2$ : pendulum hinge inertia.

$J_p$ : pendulum inertia about its center of mass, about an axis perpendicular to the swing plane.

$$\hat{J}_0 \triangleq \hat{J}_1 + m_p L_r^2$$

Rigid links; frictionless joints.

---

## 2. Parameter evaluation

Given:

$$L_r = 0.19 \text{ m}, \quad m_r = 0.051 \text{ kg}$$

$$\begin{aligned}
L_h &= 0.17 \text{ m}, & L_v &= 0.12 \text{ m} \\
m_{\text{rod, total}} &= 10.3 \text{ g} = 0.0103 \text{ kg} \\
m_s &= 7.7 \text{ g} = 0.0077 \text{ kg}, & x_s &= 0.103 \text{ m}
\end{aligned}$$

Linear density:

$$\lambda = \frac{10.3 \text{ g}}{290 \text{ mm}} = 0.03552 \text{ g/mm}$$

Mass split:

$$\begin{aligned}
m_h &= 170\lambda = 6.04 \text{ g} = 0.006038 \text{ kg} \\
m_{\text{rod}} &= 120\lambda = 4.26 \text{ g} = 0.004262 \text{ kg}
\end{aligned}$$

Swinging mass:

$$m_p = m_{\text{rod}} + m_s = 0.011962069 \text{ kg}$$

COM distance:

$$\begin{aligned}
x_{\text{rod}} &= \frac{L_v}{2} = 0.06 \text{ m} \\
l_p &= \frac{m_{\text{rod}}x_{\text{rod}} + m_sx_s}{m_p} \\
l_p &= \frac{(0.004262)(0.06) + (0.0077)(0.103)}{0.011962069} \\
l_p &= \frac{2.5572 \times 10^{-4} + 7.931 \times 10^{-4}}{0.011962069} = 0.087679158 \text{ m}
\end{aligned}$$

Pendulum hinge inertia (rod about end + sphere point mass):

$$\begin{aligned}
I_{\text{rod, piv}} &= \frac{1}{3}m_{\text{rod}}L_v^2 = \frac{1}{3}(0.004262)(0.12^2) = 2.045793103 \times 10^{-5} \\
I_{\text{s, piv}} &= m_sx_s^2 = (0.0077)(0.103^2) = 8.16893 \times 10^{-5} \\
\hat{J}_2 &= I_{\text{rod, piv}} + I_{\text{s, piv}} = 1.021472310 \times 10^{-4} \text{ kg m}^2
\end{aligned}$$

Gravity constant:

$$G = m_pg l_p = (0.011962069)(9.81)(0.087679158) = 1.028896479 \times 10^{-2} \text{ N m}$$

Coupling constant:

$$K = m_pL_rl_p = (0.011962069)(0.19)(0.087679158) = 1.992765862 \times 10^{-4} \text{ kg m}^2$$

Arm-side yaw inertia:

$$\hat{J}_0 = \hat{J}_1 + m_p L_r^2$$


---

### 3. Kinematics

Let  $\{\mathbf{i}, \mathbf{j}, \mathbf{k}\}$  be an inertial orthonormal basis. Define the planar arm basis

$$\mathbf{e}_r \equiv \cos \theta \mathbf{i} + \sin \theta \mathbf{j}, \quad \mathbf{e}_t \equiv -\sin \theta \mathbf{i} + \cos \theta \mathbf{j}$$

Arm hinge position:

$$\mathbf{r}_h = L_r \mathbf{e}_r$$

Pendulum COM relative to hinge:

$$\mathbf{r}_{p/h} = l_p (\sin \alpha \mathbf{e}_t + \cos \alpha \mathbf{k})$$

Pendulum COM position:

$$\mathbf{r}_p = \mathbf{r}_h + \mathbf{r}_{p/h}$$

Components  $\mathbf{r}_p = x\mathbf{i} + y\mathbf{j} + z\mathbf{k}$ :

$$x = L_r \cos \theta - l_p \sin \alpha \sin \theta$$

$$y = L_r \sin \theta + l_p \sin \alpha \cos \theta$$

$$z = l_p \cos \alpha$$

Derivatives:

$$\frac{d}{dt}(\cos \theta) = -\sin \theta \dot{\theta}, \quad \frac{d}{dt}(\sin \theta) = \cos \theta \dot{\theta}$$

$$\frac{d}{dt}(\sin \alpha) = \cos \alpha \dot{\alpha}, \quad \frac{d}{dt}(\cos \alpha) = -\sin \alpha \dot{\alpha}$$

### 3.1 Velocity components

For  $x$ :

$$\begin{aligned}\dot{x} &= \frac{d}{dt}(L_r \cos \theta) - l_p \frac{d}{dt}(\sin \alpha \sin \theta) \\ \frac{d}{dt}(L_r \cos \theta) &= -L_r \sin \theta \dot{\theta} \\ \frac{d}{dt}(\sin \alpha \sin \theta) &= (\cos \alpha \dot{\alpha}) \sin \theta + \sin \alpha (\cos \theta \dot{\theta}) \\ \dot{x} &= -L_r \sin \theta \dot{\theta} - l_p \cos \alpha \sin \theta \dot{\alpha} - l_p \sin \alpha \cos \theta \dot{\theta}\end{aligned}$$

For  $y$ :

$$\begin{aligned}\dot{y} &= \frac{d}{dt}(L_r \sin \theta) + l_p \frac{d}{dt}(\sin \alpha \cos \theta) \\ \frac{d}{dt}(L_r \sin \theta) &= L_r \cos \theta \dot{\theta} \\ \frac{d}{dt}(\sin \alpha \cos \theta) &= (\cos \alpha \dot{\alpha}) \cos \theta + \sin \alpha (-\sin \theta \dot{\theta}) \\ \dot{y} &= L_r \cos \theta \dot{\theta} + l_p \cos \alpha \cos \theta \dot{\alpha} - l_p \sin \alpha \sin \theta \dot{\theta}\end{aligned}$$

For  $z$ :

$$\dot{z} = \frac{d}{dt}(l_p \cos \alpha) = -l_p \sin \alpha \dot{\alpha}$$

### 3.2 Speed squared

Compute  $v^2 = \dot{x}^2 + \dot{y}^2 + \dot{z}^2$ .

Define

$$\begin{aligned}A &= L_r \sin \theta + l_p \sin \alpha \cos \theta, & B &= l_p \cos \alpha \sin \theta \\ C &= L_r \cos \theta - l_p \sin \alpha \sin \theta, & D &= l_p \cos \alpha \cos \theta\end{aligned}$$

Then

$$\dot{x} = -A\dot{\theta} - B\dot{\alpha}, \quad \dot{y} = C\dot{\theta} + D\dot{\alpha}, \quad \dot{z} = -l_p \sin \alpha \dot{\alpha}$$

Square:

$$\begin{aligned}\dot{x}^2 &= A^2 \dot{\theta}^2 + B^2 \dot{\alpha}^2 + 2AB \dot{\theta} \dot{\alpha} \\ \dot{y}^2 &= C^2 \dot{\theta}^2 + D^2 \dot{\alpha}^2 + 2CD \dot{\theta} \dot{\alpha} \\ \dot{z}^2 &= l_p^2 \sin^2 \alpha \dot{\alpha}^2\end{aligned}$$

Collect  $\dot{\theta}^2$ :

$$A^2 + C^2 = (L_r \sin \theta + l_p \sin \alpha \cos \theta)^2 + (L_r \cos \theta - l_p \sin \alpha \sin \theta)^2$$

Expand:

$$\begin{aligned} A^2 &= L_r^2 \sin^2 \theta + l_p^2 \sin^2 \alpha \cos^2 \theta + 2L_r l_p \sin \alpha \sin \theta \cos \theta, \\ C^2 &= L_r^2 \cos^2 \theta + l_p^2 \sin^2 \alpha \sin^2 \theta - 2L_r l_p \sin \alpha \sin \theta \cos \theta. \end{aligned}$$

Add:

$$A^2 + C^2 = L_r^2 (\sin^2 \theta + \cos^2 \theta) + l_p^2 \sin^2 \alpha (\sin^2 \theta + \cos^2 \theta) = L_r^2 + l_p^2 \sin^2 \alpha$$

Collect  $\dot{\alpha}^2$ :

$$B^2 + D^2 + l_p^2 \sin^2 \alpha = l_p^2 \cos^2 \alpha (\sin^2 \theta + \cos^2 \theta) + l_p^2 \sin^2 \alpha = l_p^2$$

Collect  $\dot{\theta}\dot{\alpha}$ :

$$AB + CD = l_p \cos \alpha \left[ (L_r \sin \theta + l_p \sin \alpha \cos \theta) \sin \theta + (L_r \cos \theta - l_p \sin \alpha \sin \theta) \cos \theta \right]$$

Expand bracket:

$$\begin{aligned} &(L_r \sin \theta + l_p \sin \alpha \cos \theta) \sin \theta + (L_r \cos \theta - l_p \sin \alpha \sin \theta) \cos \theta \\ &= L_r (\sin^2 \theta + \cos^2 \theta) + l_p \sin \alpha (\cos \theta \sin \theta - \sin \theta \cos \theta) = L_r. \end{aligned}$$

Thus

$$AB + CD = L_r l_p \cos \alpha$$

Therefore

$$v^2 = (L_r^2 + l_p^2 \sin^2 \alpha) \dot{\theta}^2 + l_p^2 \dot{\alpha}^2 + 2L_r l_p \cos \alpha \dot{\theta} \dot{\alpha}$$


---

#### 4. Energies

Translational kinetic energy:

$$T_{\text{trans}} = \frac{1}{2} m_p v^2$$

Rotational kinetic energy of the pendulum about its COM (perpendicular axis):

$$T_{\text{rot}} = \frac{1}{2} J_p (\dot{\alpha}^2 + \sin^2 \alpha \dot{\theta}^2)$$

Parallel axis:

$$\hat{J}_2 = J_p + m_p l_p^2$$

Arm yaw kinetic energy:

$$T_{\text{arm}} = \frac{1}{2} \hat{J}_1 \dot{\theta}^2$$

Total kinetic energy:

$$T = T_{\text{arm}} + T_{\text{trans}} + T_{\text{rot}}$$

Collect terms.

Coefficient of  $\dot{\theta}^2$ :

$$\frac{1}{2} \left[ \hat{J}_1 + m_p L_r^2 + (m_p l_p^2 + J_p) \sin^2 \alpha \right] \dot{\theta}^2 = \frac{1}{2} (\hat{J}_0 + \hat{J}_2 \sin^2 \alpha) \dot{\theta}^2$$

Coefficient of  $\dot{\alpha}^2$ :

$$\frac{1}{2} (m_p l_p^2 + J_p) \dot{\alpha}^2 = \frac{1}{2} \hat{J}_2 \dot{\alpha}^2$$

Cross term:

$$m_p L_r l_p \cos \alpha \dot{\theta} \dot{\alpha} = K \cos \alpha \dot{\theta} \dot{\alpha}$$

Thus

$$T = \frac{1}{2} (\hat{J}_0 + \hat{J}_2 \sin^2 \alpha) \dot{\theta}^2 + \frac{1}{2} \hat{J}_2 \dot{\alpha}^2 + K \cos \alpha \dot{\theta} \dot{\alpha}$$

Potential energy:

$$V = m_p g z = m_p g l_p \cos \alpha = G \cos \alpha$$

Lagrangian:

$$\mathcal{L} = T - V$$


---

## 5. Euler–Lagrange equations

$$\frac{d}{dt} \left( \frac{\partial \mathcal{L}}{\partial \dot{q}} \right) - \frac{\partial \mathcal{L}}{\partial q} = Q$$

$$Q_\theta = \tau, \quad Q_\alpha = 0$$

### 5.1 Equation in $\theta$

$$\frac{\partial \mathcal{L}}{\partial \dot{\theta}} = (\hat{J}_0 + \hat{J}_2 \sin^2 \alpha) \dot{\theta} + K \cos \alpha \dot{\alpha}$$

Differentiate:

$$\frac{d}{dt} [(\hat{J}_0 + \hat{J}_2 \sin^2 \alpha) \dot{\theta}] = (\hat{J}_0 + \hat{J}_2 \sin^2 \alpha) \ddot{\theta} + \hat{J}_2 \frac{d}{dt} (\sin^2 \alpha) \dot{\theta}$$

$$\frac{d}{dt} (\sin^2 \alpha) = 2 \sin \alpha \cos \alpha \dot{\alpha} = \sin(2\alpha) \dot{\alpha}$$

$$\frac{d}{dt} (K \cos \alpha \dot{\alpha}) = K (-\sin \alpha \dot{\alpha}^2 + \cos \alpha \ddot{\alpha})$$

Also  $\partial \mathcal{L} / \partial \theta = 0$ .

Thus

$$(\hat{J}_0 + \hat{J}_2 \sin^2 \alpha) \ddot{\theta} + K \cos \alpha \ddot{\alpha} + \hat{J}_2 \sin(2\alpha) \dot{\theta} \dot{\alpha} - K \sin \alpha \dot{\alpha}^2 = \tau$$

### 5.2 Equation in $\alpha$

$$\frac{\partial \mathcal{L}}{\partial \dot{\alpha}} = \hat{J}_2 \dot{\alpha} + K \cos \alpha \dot{\theta}$$

Differentiate:

$$\frac{d}{dt} (\hat{J}_2 \dot{\alpha}) = \hat{J}_2 \ddot{\alpha}$$

$$\frac{d}{dt} (K \cos \alpha \dot{\theta}) = K (-\sin \alpha \dot{\alpha} \dot{\theta} + \cos \alpha \ddot{\theta})$$

Partial derivative:

$$\frac{\partial \mathcal{L}}{\partial \alpha} = \frac{1}{2} \hat{J}_2 \frac{\partial}{\partial \alpha} (\sin^2 \alpha) \dot{\theta}^2 - K \sin \alpha \dot{\theta} \dot{\alpha} + G \sin \alpha$$

$$\frac{\partial}{\partial \alpha} (\sin^2 \alpha) = \sin(2\alpha)$$

Thus

$$\frac{\partial \mathcal{L}}{\partial \alpha} = \frac{1}{2} \hat{J}_2 \sin(2\alpha) \dot{\theta}^2 - K \sin \alpha \dot{\theta} \dot{\alpha} + G \sin \alpha$$

Euler–Lagrange ( $Q_\alpha = 0$ ):

$$\hat{J}_2 \ddot{\alpha} + K \cos \alpha \ddot{\theta} - K \sin \alpha \dot{\alpha} \dot{\theta} - \left( \frac{1}{2} \hat{J}_2 \sin(2\alpha) \dot{\theta}^2 - K \sin \alpha \dot{\theta} \dot{\alpha} + G \sin \alpha \right) = 0$$

Cancel the  $\pm K \sin \alpha \dot{\theta} \dot{\alpha}$  terms:

$$K \cos \alpha \ddot{\theta} + \hat{J}_2 \ddot{\alpha} - \frac{1}{2} \hat{J}_2 \sin(2\alpha) \dot{\theta}^2 - G \sin \alpha = 0$$


---

## 6. Nonlinear model

$$(\hat{J}_0 + \hat{J}_2 \sin^2 \alpha) \ddot{\theta} + K \cos \alpha \ddot{\alpha} + \hat{J}_2 \sin(2\alpha) \dot{\theta} \dot{\alpha} - K \sin \alpha \dot{\alpha}^2 = \tau$$

$$K \cos \alpha \ddot{\theta} + \hat{J}_2 \ddot{\alpha} - \frac{1}{2} \hat{J}_2 \sin(2\alpha) \dot{\theta}^2 - G \sin \alpha = 0$$

The derived equations are structurally consistent with classical Furuta pendulum models, with the distinction that actuator dynamics are treated at the acceleration level rather than torque level.

---

## 7. Linearization about upright ( $\alpha \approx 0$ )

$$\sin \alpha \approx \alpha, \quad \cos \alpha \approx 1, \quad \sin(2\alpha) \approx 2\alpha$$

Neglect products of small quantities.

Linear model:

$$\begin{aligned} \hat{J}_0 \ddot{\theta} + K \ddot{\alpha} &= \tau \\ K \ddot{\theta} + \hat{J}_2 \ddot{\alpha} - G \alpha &= 0 \end{aligned}$$

Solve for  $\ddot{\alpha}$ :

$$\ddot{\alpha} = \frac{G}{\hat{J}_2} \alpha - \frac{K}{\hat{J}_2} \ddot{\theta}$$


---



## 8. Numerical specialization

Let  $J_0 \equiv \hat{J}_0$  and  $J_1 \equiv \hat{J}_2$ . Numerical values:

$$J_0 = 0.001104 \text{ kg m}^2, \quad J_1 = 1.021 \times 10^{-4} \text{ kg m}^2, \quad K = 1.993 \times 10^{-4} \text{ kg m}^2, \quad G = 0.01029 \text{ N m}$$

Linear equations:

$$\begin{aligned} J_0 \ddot{\theta} + K \ddot{\alpha} &= \tau \\ K \ddot{\theta} + J_1 \ddot{\alpha} - G \alpha &= 0 \end{aligned}$$

Reduced relation:

$$\ddot{\alpha} = \frac{G}{J_1} \alpha - \frac{K}{J_1} \ddot{\theta}$$

Numerically:

$$\ddot{\alpha} = 100.8 \alpha - 1.952 \ddot{\theta}$$

Open-loop fall rate ( $\tau = 0$ ). From  $\ddot{\theta} = -(K/J_0)\ddot{\alpha}$ :

$$\left( J_1 - \frac{K^2}{J_0} \right) \ddot{\alpha} - G \alpha = 0$$

$$J_{eq} = J_1 - \frac{K^2}{J_0} = 0.0001021 - \frac{(0.0001993)^2}{0.001104} = 6.612 \times 10^{-5}$$

$$\ddot{\alpha} = \frac{G}{J_{eq}} \alpha, \quad \lambda = \pm \sqrt{\frac{G}{J_{eq}}} = \pm 12.47 \text{ rad/s}$$

Mass matrix inverse:

$$M = \begin{bmatrix} J_0 & K \\ K & J_1 \end{bmatrix}, \quad M^{-1} = \frac{1}{J_0 J_1 - K^2} \begin{bmatrix} J_1 & -K \\ -K & J_0 \end{bmatrix}$$

$$J_0 J_1 - K^2 = 7.2998 \times 10^{-8}$$

$$M^{-1} = \begin{bmatrix} 1398.7 & -2730.2 \\ -2730.2 & 15123.7 \end{bmatrix}$$

Substituted form:

$$0.001104 \ddot{\theta} + 0.0001993 \ddot{\alpha} = \tau$$

$$0.0001993 \ddot{\theta} + 0.0001021 \ddot{\alpha} - 0.01029 \alpha = 0$$

Nonlinear model with numerical constants:

$$(J_0 + J_1 \sin^2 \alpha) \ddot{\theta} + K \cos \alpha \ddot{\alpha} + J_1 \sin(2\alpha) \dot{\theta} \dot{\alpha} - K \sin \alpha \dot{\alpha}^2 = \tau$$

$$K \cos \alpha \ddot{\theta} + J_1 \ddot{\alpha} - \frac{1}{2} J_1 \sin(2\alpha) \dot{\theta}^2 - G \sin \alpha = 0$$


---

## 9. PD design on commanded arm acceleration

Plant:

$$\ddot{\alpha} = A\alpha - B\ddot{\theta}, \quad A \equiv \frac{G}{J_1}, \quad B \equiv \frac{K}{J_1}$$

Controller:

$$\ddot{\theta}_{cmd} = -k_p \alpha - k_d \dot{\alpha}$$

Closed-loop characteristic equation:

$$\ddot{\alpha} - (Bk_d)\dot{\alpha} - (A + Bk_p)\alpha = 0$$

Match to

$$\ddot{\alpha} + 2\zeta\omega_c\dot{\alpha} + \omega_c^2\alpha = 0$$

Gains:

$$k_d = -\frac{2\zeta\omega_c}{B}, \quad k_p = -\frac{A + \omega_c^2}{B}$$

With  $\omega_c = 15$ ,  $\zeta = 0.8$ ,  $A = 100.8$ ,  $B = 1.952$ :

$$k_p = -166.9, \quad k_d = -12.3$$

Negative gains arise from the sign convention  $\alpha = 0$  upright; the controller provides restoring acceleration opposing the unstable gravitational term.

Stepper conversion ( $N = 1600$  microsteps/rev):

$$\text{steps/rad} = \frac{N}{2\pi} = 254.65, \quad \text{steps/deg} = \frac{N}{360} = 4.444$$

Degree variables ( $\alpha_{\text{deg}} = \alpha \, 180/\pi$ ):

$$\ddot{\theta}_{\text{steps}} = -(742 \, \alpha_{\text{deg}} + 54.6 \, \dot{\alpha}_{\text{deg}})$$


---

## 10. State-space representation and LQR design

### 10.1 State definition

Define the state vector as

$$\mathbf{x} = \begin{bmatrix} x_1 \\ x_2 \\ x_3 \\ x_4 \end{bmatrix} = \begin{bmatrix} \theta \\ \alpha \\ \dot{\theta} \\ \dot{\alpha} \end{bmatrix}$$

The control input is chosen as the commanded arm angular acceleration

$$u \equiv \ddot{\theta}$$


---

### 10.2 Linearized state-space model

The state equations are

$$\begin{aligned} \dot{x}_1 &= x_3 \\ \dot{x}_2 &= x_4 \\ \dot{x}_3 &= u \\ \dot{x}_4 &= A x_2 - B u \end{aligned}$$

where

$$A \equiv \frac{G}{J_1}, \quad B \equiv \frac{K}{J_1}$$

Collecting terms, the state-space model is

$$\dot{\mathbf{x}} = \mathbf{A}\mathbf{x} + \mathbf{B}u$$

with

$$\mathbf{A} = \begin{bmatrix} 0 & 0 & 1 & 0 \\ 0 & 0 & 0 & 1 \\ 0 & 0 & 0 & 0 \\ 0 & A & 0 & 0 \end{bmatrix}, \quad \mathbf{B} = \begin{bmatrix} 0 \\ 0 \\ 1 \\ -B \end{bmatrix}$$

Numerically,

$$\mathbf{A} = \begin{bmatrix} 0 & 0 & 1 & 0 \\ 0 & 0 & 0 & 1 \\ 0 & 0 & 0 & 0 \\ 0 & 100.8 & 0 & 0 \end{bmatrix}, \quad \mathbf{B} = \begin{bmatrix} 0 \\ 0 \\ 1 \\ -1.952 \end{bmatrix}$$


---

### 10.3 LQR formulation

A continuous-time linear quadratic regulator (LQR) is designed with the control law

$$u = -\mathbf{K}\mathbf{x}$$

minimizing the cost function

$$J = \int_0^\infty (\mathbf{x}^\top \mathbf{Q} \mathbf{x} + u^\top \mathbf{R} u) dt$$


---

### 10.4 LQR gain

The gain is computed by solving the continuous-time algebraic Riccati equation (CARE)

$$\mathbf{A}^\top \mathbf{P} + \mathbf{P} \mathbf{A} - \mathbf{P} \mathbf{B} \mathbf{R}^{-1} \mathbf{B}^\top \mathbf{P} + \mathbf{Q} = \mathbf{0}$$

and then

$$\mathbf{K} = \mathbf{R}^{-1} \mathbf{B}^\top \mathbf{P}.$$

For the numerical gain below, the weights are

$$\mathbf{Q} = \text{diag}(0.5, 50.0, 0.05, 5.0), \quad \mathbf{R} = [1.0].$$

This choice prioritizes pendulum angle stabilization (large weight on  $\alpha$ ) while penalizing control effort.

Numerical values are obtained by solving the CARE (e.g., via SciPy `solve_continuous_are`) and evaluating  $\mathbf{K} = \mathbf{R}^{-1} \mathbf{B}^\top \mathbf{P}$ .

$$\mathbf{K} = [-0.70710678 \quad -117.18259227 \quad -1.3583044 \quad -11.86304115]$$

The resulting control law is

$$u = -(-0.7071 \theta - 117.183 \alpha - 1.3583 \dot{\theta} - 11.8630 \dot{\alpha})$$

Stepper units using degree variables. Let

$$\mathbf{x}_{\text{deg}} = \begin{bmatrix} \theta_{\text{deg}} \\ \alpha_{\text{deg}} \\ \dot{\theta}_{\text{deg}} \\ \dot{\alpha}_{\text{deg}} \end{bmatrix}, \quad \mathbf{x} = \frac{\pi}{180} \mathbf{x}_{\text{deg}}$$

Let  $u_{\text{deg}} \equiv \ddot{\theta}_{\text{deg}}$  denote acceleration in  $\text{deg/s}^2$ , so that  $u = (\pi/180)u_{\text{deg}}$ . Then

$$\ddot{\theta}_{\text{steps}} = \frac{N}{2\pi} u = \frac{N}{360} u_{\text{deg}}$$

Then

$$\ddot{\theta}_{\text{steps}} = -\mathbf{K}_{\text{steps}} \mathbf{x}_{\text{deg}}$$

$$\mathbf{K}_{\text{steps}} = \left( \frac{N}{360} \right) \mathbf{K} = 4.444 \mathbf{K} = \begin{bmatrix} -3.1424 & -520.76 & -6.0363 & -52.72 \end{bmatrix}$$

$$\ddot{\theta}_{\text{steps}} = -(-3.1424 \theta_{\text{deg}} - 520.76 \alpha_{\text{deg}} - 6.0363 \dot{\theta}_{\text{deg}} - 52.72 \dot{\alpha}_{\text{deg}})$$


---